coq/ModuleAssumptions.v
@@ -22,6 +22,7 @@ Inductive is_supported_ibinop : ibinop -> Prop :=
 
 Inductive is_supported_shift : ibinop -> Prop :=
   | IS_Shl : is_supported_shift (Shl false false)
+  | IS_LShr : is_supported_shift (LShr false)
 .
 
 Inductive is_supported_conv : conversion_type -> Prop :=
